<?xml version="1.0" encoding="ISO-8859-1" standalone="yes"?>

<!DOCTYPE rdf:RDF [
   <!ENTITY rdf "http://www.w3.org/1999/02/22-rdf-syntax-ns#">
   <!ENTITY rdfs "http://www.w3.org/2000/01/rdf-schema#">
   <!ENTITY owl "http://www.w3.org/2002/07/owl#">
   <!ENTITY s2   "http://www.esa.int/s2#">
   <!ENTITY drb "http://www.gael.fr/drb#">
   <!ENTITY jpeg2000 "http://www.gael.fr/drb/jpeg2000#">
]>

<rdf:RDF xmlns:owl="&owl;"
         xmlns:rdf="&rdf;"
         xmlns:rdfs="&rdfs;"
         xmlns:drb="&drb;"
         xmlns:jpeg2000="&jpeg2000;"
         xmlns:s2="&s2;"
         xml:base="&s2;">

<!--
* Data Hub Service (DHuS) - For Space data distribution.
* Copyright (C) 2013,2014,2015,2016 GAEL Systems
*
* This file is part of DHuS software sources.
*
* This program is free software: you can redistribute it and/or modify
* it under the terms of the GNU Affero General Public License as
* published by the Free Software Foundation, either version 3 of the
* License, or (at your option) any later version.
*
* This program is distributed in the hope that it will be useful,
* but WITHOUT ANY WARRANTY; without even the implied warranty of
* MERCHANTABILITY or FITNESS FOR A PARTICULAR PURPOSE. See the
* GNU Affero General Public License for more details.
*
* You should have received a copy of the GNU Affero General Public License
* along with this program. If not, see <http://www.gnu.org/licenses/>.
-->

   <owl:Ontology rdf:about="&s2;">
      <rdfs:label xml:lang="en">Sentinel-2 Level-1A Ontology</rdfs:label>
   </owl:Ontology>

   <!-- ========================================= -->
   <!-- User Level-1A Product                     -->
   <!-- ========================================= -->

   <!-- WARN ID changed
        <owl:Class rdf:about="&s2;userLevel1AProduct"> -->
   <owl:Class rdf:about="&s2;userProductLevel1a">
      <rdfs:label xml:lang="en">Sentinel-2 User Product Level-1A</rdfs:label>
      <rdfs:comment xml:lang="en">
         Level-1A product is obtained by decompressing image data and
         developing a geometric model to locate any pixel in the image.
         The following list introduces the input data of Level-1A processing:
         * Input of Level-1A processing - Metadata: Metadata from Level-0
         product.
         * Input of Level-1A processing - Image Data: Level-0 data
         (granules).
         * Input of Level-1A processing - Auxiliary Data: GIPP: Parameters from
         Level-0 complemented by radiometric and geometric processing
         parameters. DEM: only the reference to the data used is provided.
         * Input of Level-1A processing - Quality Indicator Data: Quality
         indicators from Level-0.
         This level corresponds to the systematic processing steps that must be
         applied before any further processing. It includes:
         * decompression of the image data,
         * geometric model computation : geolocation information, coarse
         interband / interdetector registration,
         * SWIR pixels re-arrangement.
         As requiring only a fast processing, this 'Raw Level' product can be
         used to allow a quick display of the detectors (sub-swaths) in full
         resolution. The sub swath can be displayed using standard commercial
         image processing software.
         Note that one Level-1A product:
         * refers always to one Datatake;
         * refer to one or several DataStrip from the same Datatake;
         * may cover the full Datatake or an extract of the Datatake.
         In the case of an extract, image data is provided only to cover the
         selected extract but the ancillary data are always provided through a
         metadata file on the temporal extent of the full Datatake.
         The Level-1A User product consists of:
         1. Product_Metadata_File: This is the mandatory XML main metadata file
         (DIMAP) containing the requested level of information and referring
         all the product elements.
         2. manifest.safe: this is the SAFE metadata file (optional). It is
         included in the product only if the user requests the product to be
         SAFE formatted (according to a specific download option).
         3. GRANULE: folder containing all granules composing the product
         (Image Data). The Image data are provided by a set of raster files.
         The image data extent correspond to a set of .'granules.' and can
         covers up to 12 detectors * 13 bands of the orbit in full resolution.
         A sub-set of the 13 bands can be provided.
         4. DATASTRIP: folder containing the DataStrip composing the product
         linked to the selected granules.
         5. AUX_DATA: folder containing the auxiliary data items needed for the
         Level-1A processing and provided with the product on request by the
         user. Some auxiliary data (for instance IERS Bullettin and GIPPs
         files) can be provided either with the product (if selected by the
         user according to a specific download option) or external to the
         product (referenced through the Product_Metadata_File), others are
         only external to the product (for instance the DEM used for the
         processing); in any case, all the auxiliary data files are referenced
         in the XML Main metadata file.
         6. rep_info: folder containing the XSD schema provided inside the
         product. This folder is optional. It will be included in the final
         product if the user select the SAFE format as output format.
         7. Preview_Image: file consisting of an image limited to 3
         visible-bands in ground geometry at 320m resolution. This file,
         provided if requested by the user, gives an overview of the product
         (sub-sampled) mainly for image data browsing and selection purposes,
         8. INSPIRE: XML INSPIRE metadata file.
      </rdfs:comment>
       <rdfs:subClassOf rdf:resource="&s2;userProduct"/>
      <drb:signature rdf:parseType="Resource">
         <drb:nameMatch>S2[AB]_...._PRD_MSIL1A_PDMC_[0-9]{4}[0-1][0-9][0-3][0-9]T[0-2][0-9][0-6][0-9][0-6][0-9]_R[0-9]{3}_V[0-9]{4}[0-1][0-9][0-3][0-9]T[0-2][0-9][0-6][0-9][0-6][0-9]_[0-9]{4}[0-1][0-9][0-3][0-9]T[0-2][0-9][0-6][0-9][0-6][0-9]\.SAFE</drb:nameMatch>
      </drb:signature>
   </owl:Class>

   <!-- ========================================= -->
   <!-- Metadata File (Level-1A)                  -->
   <!-- ========================================= -->

   <owl:Class rdf:about="&s2;userProductLevel1aMetadataFile">
      <rdfs:label xml:lang="en">User Product Level-1A: Metadata File</rdfs:label>
      <rdfs:comment xml:lang="en">
         The XML metadata file provided inside the S2 Level-1A User Product.
      </rdfs:comment>
      <rdfs:subClassOf rdf:resource="&drb;xml"/>
      <drb:signature rdf:parseType="Resource">
         <drb:parentIsSubClassTest>&s2;userProduct</drb:parentIsSubClassTest>
         <drb:nameMatch>S2[AB]_...._MTD_(SAF|DMP)L1A_PDMC.*</drb:nameMatch>
      </drb:signature>
      <!-- This xsd is in the product, but in the repository too -->
      <drb:schemaLocation>
          xsd/int/esa/sentinel-2/S2_User_Product_Level-1A_Metadata.xsd
      </drb:schemaLocation>
   </owl:Class>

   <!-- ========================================= -->
   <!-- Metadata XSD (Level-1A)                   -->
   <!-- ========================================= -->

   <owl:Class rdf:about="&s2;userProductLevel1aMetadataXsd">
      <rdfs:label xml:lang="en">User Product Level-1A: Metadata XML Schema</rdfs:label>
      <rdfs:comment xml:lang="en">
         The XML schema describing the metadata file provided inside the S2
         Level-1A User Product.
      </rdfs:comment>
      <rdfs:subClassOf rdf:resource="&drb;item"/>
      <drb:signature rdf:parseType="Resource">
         <drb:parentClassTest>&s2;representationInformationFolder</drb:parentClassTest>
         <drb:nameMatch>S2_User_Product_Level-1A_Metadata.xsd</drb:nameMatch>
      </drb:signature>
   </owl:Class>

   <!-- ========================================= -->
   <!-- Granule (Level-1A)                        -->
   <!-- ========================================= -->

   <!-- WARN ID changed
       <owl:Class rdf:about="&s2;pdi_level_1a_granule_container"> -->
   <owl:Class rdf:about="&s2;level1aGranule">
      <rdfs:label xml:lang="en">Level-1A Granule</rdfs:label>
      <rdfs:comment xml:lang="en">
         One of the granules composing the User Product Level-1A.
         The PDI Level-1A granule consists of:
         1. Level-1A_Granule_Metadata_File: XML metadata file containing the
            requested level of information and referring all the product
            elements composing the Granule;
         2. IMG_DATA: folder containing image data compressed using the JPEG2000
            algorithm, one file per spectral band;
         3. QI_DATA: folder containing XML reports including Quality control
            checks and Quality Mask files;
         4. Inventory_Metadata.xml: file containing the metadata needed to
            inventory the PDI;
         5. manifest.safe: XML SAFE Manifest file;
         6. rep_info: folder containing the available XSD schemas that
            validate the PDI components.
         Note that the Inventory_Metadata.xml, manifest.safe and rep_info are
         available inside a Granule but they are removed when the PDI is
         included in the User Product.
      </rdfs:comment>
      <rdfs:subClassOf rdf:resource="&s2;granule"/>
      <drb:signature rdf:parseType="Resource">
         <drb:parentClassTest>&s2;granuleWrapper</drb:parentClassTest>
         <drb:nameMatch>S2[AB]_...._MSI_L1A_GR.*_N[0-9]{2}\.[0-9]{2}</drb:nameMatch>
      </drb:signature>
   </owl:Class>

   <!-- ========================================= -->
   <!-- Granule Image File (Level-1A)             -->
   <!-- ========================================= -->

   <!-- WARN ID changed
        <owl:Class rdf:about="&s2;pdi_level_1a_image_file"> -->
   <owl:Class rdf:about="&s2;level1aImageFile">
      <rdfs:label xml:lang="en">Level-1A Image File</rdfs:label>
      <rdfs:comment xml:lang="en">
         One JPEG2000 file per band.
      </rdfs:comment>
      <rdfs:subClassOf rdf:resource="&jpeg2000;JPEG2000"/>
      <drb:signature rdf:parseType="Resource">
         <drb:parentClassTest>&s2;imageFolder</drb:parentClassTest>
         <drb:nameMatch>S2[AB]_...._MSI_L1A_.*_B(01|02|03|04|05|06|07|08|09|10|11|12|8A)\.(?i)jp2</drb:nameMatch>
      </drb:signature>
   </owl:Class>

   <!-- ========================================= -->
   <!-- Granule Metadata File (Level-1A)          -->
   <!-- ========================================= -->

   <!-- WARN ID changed
        <owl:Class rdf:about="&s2;pdi_level_1a_granule_metadata"> -->
   <owl:Class rdf:about="&s2;level1aGranuleMetadataFile">
      <rdfs:label xml:lang="en">Level-1A Granule Metadata File</rdfs:label>
      <rdfs:comment xml:lang="en">
         The XML metadata file provided inside each Level-1A granule.
      </rdfs:comment>
      <rdfs:subClassOf rdf:resource="&s2;granuleMetadataFile"/>
      <drb:signature rdf:parseType="Resource">
         <drb:parentClassTest>&s2;level1aGranule</drb:parentClassTest>
         <drb:nameMatch>S2[AB]_...._MTD_L1A_GR_.*</drb:nameMatch>
      </drb:signature>
      <drb:schemaLocation>xsd/int/esa/sentinel-2/S2_PDI_Level-1A_Granule_Metadata.xsd</drb:schemaLocation>
   </owl:Class>

   <!-- ========================================= -->
   <!-- Datastrip (Level-1A)                      -->
   <!-- ========================================= -->

   <!-- WARN ID changed
        <owl:Class rdf:about="&s2;pdi_level_1a_datastrip_container"> -->
   <owl:Class rdf:about="&s2;level1aDatastrip">
      <rdfs:label xml:lang="en">Level-1A Datastrip</rdfs:label>
      <rdfs:comment xml:lang="en">
         One of the datastrips for User Product Level-1A.
         The PDI Level-1A Datastrip consists of:
         1. Datastrip_Metadata_File: XML metadata file containing the requested
            level of information and referring all the product elements
            composing the Datastrip;
         2. QI_DATA: folder containing XML reports about Quality control checks
            information;
         3. Inventory_Metadata.xml: file containing the metadata needed to
            inventory the PDI;
         4. manifest.safe: XML SAFE Manifest file;
         5. rep_info: folder containing the available XSD schemas that validate
            the PDI components.
         Note that the Inventory_Metadata.xml, manifest.safe and rep_info are
         available inside a Datastrip but they are removed when the PDI is
         included in the User Product.
      </rdfs:comment>
      <rdfs:subClassOf rdf:resource="&s2;datastrip"/>
      <drb:signature rdf:parseType="Resource">
         <drb:parentClassTest>&s2;datastripWrapper</drb:parentClassTest>
         <drb:nameMatch>S2[AB]_...._MSI_L1A_DS.*_N[0-9]{2}\.[0-9]{2}</drb:nameMatch>
      </drb:signature>
   </owl:Class>

   <!-- ========================================= -->
   <!-- Datastrip Metadata File (Level-1A)        -->
   <!-- ========================================= -->

   <!-- WARN ID changed
        <owl:Class rdf:about="&s2;pdi_level_1a_datastrip_metadata"> -->
   <owl:Class rdf:about="&s2;level1aDatastripMetadataFile">
      <rdfs:label xml:lang="en">Level-1A Datastrip Metadata File</rdfs:label>
      <rdfs:comment xml:lang="en">
         XML Metadata file (DIMAP mandatory file) containing the requested
         level of information and referring all the product elements describing
         the datastrip.
      </rdfs:comment>
      <rdfs:subClassOf rdf:resource="&s2;datastripMetadataFile"/>
      <drb:signature rdf:parseType="Resource">
         <drb:parentClassTest>&s2;level1aDatastrip</drb:parentClassTest>
         <drb:nameMatch>S2[AB]_...._MTD_L1A_DS_.*</drb:nameMatch>
      </drb:signature>
      <drb:schemaLocation>xsd/int/esa/sentinel-2/S2_PDI_Level-1A_Datastrip_Metadata.xsd</drb:schemaLocation>
   </owl:Class>

</rdf:RDF>
