<?xml version="1.0" encoding="ISO-8859-1" standalone="yes"?>

<!DOCTYPE rdf:RDF [
   <!ENTITY rdf "http://www.w3.org/1999/02/22-rdf-syntax-ns#">
   <!ENTITY rdfs "http://www.w3.org/2000/01/rdf-schema#">
   <!ENTITY owl "http://www.w3.org/2002/07/owl#">
   <!ENTITY s2   "http://www.esa.int/s2#">
   <!ENTITY drb "http://www.gael.fr/drb#">
   <!ENTITY jpeg2000 "http://www.gael.fr/drb/jpeg2000#">
]>

<rdf:RDF xmlns:owl="&owl;"
         xmlns:rdf="&rdf;"
         xmlns:rdfs="&rdfs;"
         xmlns:drb="&drb;"
         xmlns:jpeg2000="&jpeg2000;"
         xmlns:s2="&s2;"
         xml:base="&s2;">

<!--
* Data Hub Service (DHuS) - For Space data distribution.
* Copyright (C) 2013,2014,2015,2016 GAEL Systems
*
* This file is part of DHuS software sources.
*
* This program is free software: you can redistribute it and/or modify
* it under the terms of the GNU Affero General Public License as
* published by the Free Software Foundation, either version 3 of the
* License, or (at your option) any later version.
*
* This program is distributed in the hope that it will be useful,
* but WITHOUT ANY WARRANTY; without even the implied warranty of
* MERCHANTABILITY or FITNESS FOR A PARTICULAR PURPOSE. See the
* GNU Affero General Public License for more details.
*
* You should have received a copy of the GNU Affero General Public License
* along with this program. If not, see <http://www.gnu.org/licenses/>.
-->

   <owl:Ontology rdf:about="&s2;">
      <rdfs:label xml:lang="en">Sentinel-2 Level-1C Ontology</rdfs:label>
   </owl:Ontology>

   <!-- ========================================= -->
   <!-- User Level-1C Product                     -->
   <!-- ========================================= -->

   <!-- WARN ID changed
        <owl:Class rdf:about="&s2;userLevel1CProduct"> -->
   <!-- Compliant with COMPACT -->
   <owl:Class rdf:about="&s2;userProductLevel1c">
      <rdfs:label xml:lang="en">Sentinel-2 User Product Level-1C</rdfs:label>
      <rdfs:comment xml:lang="en">
         Level-1C is an orthoimage product, i.e. a map projection of the
         acquired image using a system DEM to correct ground geometric
         distortions. Pixel radiometric measurements are provided in
         Top-Of-Atmosphere (TOA) reflectances with all parameters to transform
         them into radiances.
         Level-1C products are resampled with a constant GSD (Ground Sampling
         Distance) of 10m, 20m, 60m according to the native resolution of the
         different spectral bands.
         The following list introduces the input data of Level-1C processing:
         * Input of Level-1C processing - Metadata: Metadata from Level-1B
         product.
         * Input of Level-1C processing - Image Data: Radiometrically and
         geometrically corrected image data.
         * Input of Level-1C processing - Ancillary Data: Ancillary data from
         the Level-1B (satellite and ground ancillary data, including the
         refined geometric model).
         * Input of Level-1C processing - Auxiliary Data: GIPP: Parameters from
         Level-1B complemented by radiometric and geometric processing
         parameters.
         * Input of Level-1C processing - Quality Indicator Data: Quality
         indicator files from Level-1B.
         Note that one Level-1C product:
         * refers always to one Datatake;
         * refer to one or several Datastrip from the same Datatake;
         * may cover the full Datatake or an extract of the Datatake.
         In the case of an extract, the image data are provided to cover the
         selected extract only. In any case (full or extract of Datatake), the
         ancillary data, referenced through the product metadata file, are
         always provided on the temporal extent of the full Datatake.
         By default, Level-1C is geometrically refined. Some Level-1C may not
         be geometrically refined (e.g. for Cal/Val purposes). These products
         are identified with a dedicated flag in the metadata.
         The Level-1C User product consists of:
         1. Product_Metadata_File: This is the mandatory XML main metadata file
         (DIMAP) containing the requested level of information and referring
         all the product elements.
         2. manifest.safe: this is the SAFE metadata file (optional). It is
         included in the product only if the user requests the product to be
         SAFE formatted (according to a specific download option).
         3. GRANULE: this folder (the name is chosen for homogeneity with
         respect to the other user product) contains the tiles composing the
         product (Image Data).
         4. DATASTRIP: folder containing the Datastrip composing the product
         linked to the selected tiles.
         5. AUX_DATA: folder containing the auxiliary data items used for the
         Level-1C processing. GIPP files and IERS bulletin are provided with
         the product only if requested by the user. In addition, the Level-1C
         embeds always an elementary set of meteorological datasets extracted
         and resampled from ECMWF forecast output. In any case, all the
         auxiliary data files are referenced in the XML Main metadata file .
         6. Preview_Image: file consisting of an image limited to 3
         visible-bands in ground geometry at 320m resolution. This file,
         provided if requested by the user, gives an overview of the product
         (sub-sampled) mainly for image data browsing and selection purposes,
         7. rep_info: folder containing the XSD schema provided inside the
         product. This folder is optional. It will be included in the final
         product if the user select the SAFE format as output format.
         8. INSPIRE: XML INSPIRE metadata file.
      </rdfs:comment>
       <rdfs:subClassOf rdf:resource="&s2;userProduct"/>
      <drb:signature rdf:parseType="Resource">
         <drb:nameMatch>S2[AB]_(...._PRD_MSIL1C_PDMC_[0-9]{4}[0-1][0-9][0-3][0-9]T[0-2][0-9][0-6][0-9][0-6][0-9]_R[0-9]{3}_V[0-9]{4}[0-1][0-9][0-3][0-9]T[0-2][0-9][0-6][0-9][0-6][0-9]_[0-9]{4}[0-1][0-9][0-3][0-9]T[0-2][0-9][0-6][0-9][0-6][0-9]|MSIL.._[0-9]{4}[0-1][0-9][0-3][0-9]T[0-2][0-9][0-6][0-9][0-6][0-9]_N...._R[0-9]{3}.*)\.SAFE</drb:nameMatch>
      </drb:signature>
   </owl:Class>

   <!-- ========================================= -->
   <!-- Metadata File (Level-1C)                  -->
   <!-- ========================================= -->

   <!-- Compliant with COMPACT -->
   <owl:Class rdf:about="&s2;userProductLevel1cMetadataFile">
      <rdfs:label xml:lang="en">User Product Level-1C: Metadata File</rdfs:label>
      <rdfs:comment xml:lang="en">
         The XML metadata file provided inside the S2 Level-1C User Product.
      </rdfs:comment>
      <rdfs:subClassOf rdf:resource="&drb;xml"/>
      <drb:signature rdf:parseType="Resource">
         <drb:parentIsSubClassTest>&s2;userProduct</drb:parentIsSubClassTest>
         <drb:nameMatch>(S2[AB]_...._MTD_(SAF|DMP)L1C_PDMC.*|MTD_MSIL1C.*)</drb:nameMatch>
      </drb:signature>
      <!-- This xsd is in the product, but in the repository too -->
      <drb:schemaLocation>
          xsd/int/esa/sentinel-2/S2_User_Product_Level-1C_Metadata.xsd
      </drb:schemaLocation>
   </owl:Class>

   <!-- ========================================= -->
   <!-- Metadata XSD (Level-1C)                   -->
   <!-- ========================================= -->

   <!-- Compliant with COMPACT -->
   <owl:Class rdf:about="&s2;userProductLevel1cMetadataXsd">
      <rdfs:label xml:lang="en">User Product Level-1C: Metadata XML Schema</rdfs:label>
      <rdfs:comment xml:lang="en">
         The XML schema describing the metadata file provided inside the S2
         Level-1C User Product.
      </rdfs:comment>
      <rdfs:subClassOf rdf:resource="&drb;item"/>
      <drb:signature rdf:parseType="Resource">
         <drb:parentClassTest>&s2;representationInformationFolder</drb:parentClassTest>
         <drb:nameMatch>S2_User_Product_Level-1C_Metadata.xsd</drb:nameMatch>
      </drb:signature>
   </owl:Class>

   <!-- ========================================= -->
   <!-- Granule (Level-1C)                        -->
   <!-- ========================================= -->

   <!-- WARN ID changed
        <owl:Class rdf:about="&s2;pdi_level_1c_tile_container"> -->
   <!-- Compliant with COMPACT -->
   <owl:Class rdf:about="&s2;level1cGranule">
      <rdfs:label xml:lang="en">Level-1C Granule</rdfs:label>
      <rdfs:comment xml:lang="en">
         One of the granules composing the User Product Level-1C.
         There are N granules-folders each one corresponding to the Tiles
         composing the product.
         The PDI Level-1C Granule/Tile consists of:
         1. Level-1C_Tile_Metadata_File (Tile Metadata): XML Main Metadata
             file (DIMAP mandatory file) containing the requested level of
             information and referring all the product elements describing the
             tile,
         2. IMG_DATA: folder containing image data files compressed using the
            JPEG2000 algorithm, one file per band.
         3. QI_DATA: folder containing OLQC XML reports of quality checks, mask
            files and PVI file;
         4. Inventory_Metadata.xml: file containing the metadata needed to
            inventory the PDI;
         5. manifest.safe: XML SAFE Manifest file;
         6. rep_info: folder containing the available XSD schemas that
            validate the PDI components.
         Note that the Inventory_Metadata.xml, manifest.safe and rep_info are
         available inside a Granule but they are removed when the PDI is
         included in the User Product.
      </rdfs:comment>
      <rdfs:subClassOf rdf:resource="&s2;granule"/>
      <drb:signature rdf:parseType="Resource">
         <drb:parentClassTest>&s2;granuleWrapper</drb:parentClassTest>
         <drb:nameMatch>(S2[AB]_...._MSI_L1C_TL.*_N[0-9]{2}\.[0-9]{2}|L1C_T....._A[0-9]{6}_[0-9]{4}[0-1][0-9][0-3][0-9]T[0-2][0-9][0-6][0-9][0-6][0-9])</drb:nameMatch>
      </drb:signature>
   </owl:Class>

   <!-- ========================================= -->
   <!-- Tile Image File (Level-1C)                -->
   <!-- ========================================= -->

   <!-- WARN ID changed
        <owl:Class rdf:about="&s2;pdi_level_1c_image_file"> -->
   <!-- Compliant with COMPACT -->
   <owl:Class rdf:about="&s2;level1cTileImageFile">
      <rdfs:label xml:lang="en">Level-1C Tile Image File</rdfs:label>
      <rdfs:comment xml:lang="en">
         One JPEG2000 file per band.
      </rdfs:comment>
      <rdfs:subClassOf rdf:resource="&jpeg2000;JPEG2000"/>
      <drb:signature rdf:parseType="Resource">
         <drb:parentClassTest>&s2;imageFolder</drb:parentClassTest>
         <drb:nameMatch>(S2[AB]_...._MSI_L1C_.*|T....._[0-9]{4}[0-1][0-9][0-3][0-9]T[0-2][0-9][0-6][0-9][0-6][0-9])_(B(01|02|03|04|05|06|07|08|09|10|11|12|8A)|TCI|PVI)\.(?i)jp2</drb:nameMatch>
      </drb:signature>
   </owl:Class>

   <!-- ========================================= -->
   <!-- Tile Metadata File (Level-1C)             -->
   <!-- ========================================= -->

   <!-- WARN ID changed
        <owl:Class rdf:about="&s2;pdi_level_1c_tile_metadata"> -->
   <!-- Compliant with COMPACT -->
   <owl:Class rdf:about="&s2;level1cGranuleMetadataFile">
      <rdfs:label xml:lang="en">Level-1C Granule Metadata File</rdfs:label>
      <rdfs:comment xml:lang="en">
         The XML metadata file provided inside each Level-1C tile.
      </rdfs:comment>
      <rdfs:subClassOf rdf:resource="&s2;granuleMetadataFile"/>
      <drb:signature rdf:parseType="Resource">
         <drb:parentClassTest>&s2;level1cGranule</drb:parentClassTest>
         <drb:nameMatch>(S2[AB]_...._MTD_L1C_TL_.*|MTD_TL\.xml)</drb:nameMatch>
      </drb:signature>
      <drb:schemaLocation>xsd/int/esa/sentinel-2/S2_PDI_Level-1C_Tile_Metadata.xsd</drb:schemaLocation>
   </owl:Class>

   <!-- ========================================= -->
   <!-- Datastrip (Level-1C)                      -->
   <!-- ========================================= -->

   <!-- WARN ID changed
        <owl:Class rdf:about="&s2;pdi_level_1c_datastrip_container"> -->
   <!-- Compliant with COMPACT -->
   <owl:Class rdf:about="&s2;level1cDatastrip">
      <rdfs:label xml:lang="en">Level-1C Datastrip</rdfs:label>
      <rdfs:comment xml:lang="en">
         One of the datastrips for User Product Level-1C.
         The PDI Level 1C DataStrip consists of:
         1. DataStrip_Metadata_File: XML Main Metadata file (DIMAP mandatory
            file) containing the requested level of information and referring all
            the product elements describing the DataStrip.
         2. QI_DATA: folder containing XML reports providing Quality control
            checks information.
         4. Inventory_Metadata.xml: file containing the metadata needed to
            inventory the PDI;
         5. manifest.safe: XML SAFE Manifest file;
         6. rep_info: folder containing the available XSD schemas that
            validate the PDI components.
         Note that the Inventory_Metadata.xml, manifest.safe and rep_info are
         available inside a Datastrip but they are removed when the PDI is
         included in the User Product.
      </rdfs:comment>
      <rdfs:subClassOf rdf:resource="&s2;datastrip"/>
      <drb:signature rdf:parseType="Resource">
         <drb:parentClassTest>&s2;datastripWrapper</drb:parentClassTest>
         <drb:nameMatch>(S2[AB]_...._MSI_L1C_DS.*_N[0-9]{2}\.[0-9]{2}|DS_...._[0-9]{4}[0-1][0-9][0-3][0-9]T[0-2][0-9][0-6][0-9][0-6][0-9]_S[0-9]{4}[0-1][0-9][0-3][0-9]T[0-2][0-9][0-6][0-9][0-6][0-9])</drb:nameMatch>
      </drb:signature>
   </owl:Class>

   <!-- ========================================= -->
   <!-- Datastrip Metadata File (Level-1C)        -->
   <!-- ========================================= -->

   <!-- WARN ID changed
        <owl:Class rdf:about="&s2;pdi_level_1c_datastrip_metadata"> -->
   <!-- Compliant with COMPACT -->
   <owl:Class rdf:about="&s2;level1cDatastripMetadataFile">
      <rdfs:label xml:lang="en">Level-1C Datastrip Metadata File</rdfs:label>
      <rdfs:comment xml:lang="en">
         XML Metadata file (DIMAP mandatory file) containing the requested
         level of information and referring all the product elements describing
         the datastrip.
      </rdfs:comment>
      <rdfs:subClassOf rdf:resource="&s2;datastripMetadataFile"/>
      <drb:signature rdf:parseType="Resource">
         <drb:parentClassTest>&s2;level1cDatastrip</drb:parentClassTest>
         <drb:nameMatch>(S2[AB]_...._MTD_L1C_DS_.*|MTD_DS.*)</drb:nameMatch>
      </drb:signature>
      <drb:schemaLocation>xsd/int/esa/sentinel-2/S2_PDI_Level-1C_Datastrip_Metadata.xsd</drb:schemaLocation>
   </owl:Class>

</rdf:RDF>
