<?xml version="1.0" encoding="ISO-8859-1" standalone="yes"?>

<!DOCTYPE rdf:RDF [
   <!ENTITY rdf "http://www.w3.org/1999/02/22-rdf-syntax-ns#">
   <!ENTITY rdfs "http://www.w3.org/2000/01/rdf-schema#">
   <!ENTITY owl "http://www.w3.org/2002/07/owl#">
   <!ENTITY s2   "http://www.esa.int/s2#">
   <!ENTITY drb "http://www.gael.fr/drb#">
   <!ENTITY jpeg2000 "http://www.gael.fr/drb/jpeg2000#">
]>

<rdf:RDF xmlns:owl="&owl;"
         xmlns:rdf="&rdf;"
         xmlns:rdfs="&rdfs;"
         xmlns:drb="&drb;"
         xmlns:jpeg2000="&jpeg2000;"
         xmlns:s2="&s2;"
         xml:base="&s2;">

<!--
* Data Hub Service (DHuS) - For Space data distribution.
* Copyright (C) 2013,2014,2015,2016 GAEL Systems
*
* This file is part of DHuS software sources.
*
* This program is free software: you can redistribute it and/or modify
* it under the terms of the GNU Affero General Public License as
* published by the Free Software Foundation, either version 3 of the
* License, or (at your option) any later version.
*
* This program is distributed in the hope that it will be useful,
* but WITHOUT ANY WARRANTY; without even the implied warranty of
* MERCHANTABILITY or FITNESS FOR A PARTICULAR PURPOSE. See the
* GNU Affero General Public License for more details.
*
* You should have received a copy of the GNU Affero General Public License
* along with this program. If not, see <http://www.gnu.org/licenses/>.
-->

   <owl:Ontology rdf:about="&s2;">
      <rdfs:label xml:lang="en">Sentinel-2 Level-2A Ontology</rdfs:label>
   </owl:Ontology>

   <!-- ========================================= -->
   <!-- User Level-2A Product                     -->
   <!-- ========================================= -->

   <!-- WARN ID changed
        <owl:Class rdf:about="&s2;userLevel2AProduct"> -->
   <!-- Back to previous ID for compatibility
   <owl:Class rdf:about="&s2;userProductLevel2a">-->
   <owl:Class rdf:about="&s2;userLevel2AProduct">
      <rdfs:label xml:lang="en">Sentinel-2 User Product Level-2A</rdfs:label>
      <rdfs:comment xml:lang="en">
         TODO
      </rdfs:comment>
       <rdfs:subClassOf rdf:resource="&s2;userProduct"/>
      <drb:signature rdf:parseType="Resource">
         <drb:nameMatch>S2[AB]_(...._PRD_MSIL2A_PDMC_[0-9]{4}[0-1][0-9][0-3][0-9]T[0-2][0-9][0-6][0-9][0-6][0-9]_R[0-9]{3}_V[0-9]{4}[0-1][0-9][0-3][0-9]T[0-2][0-9][0-6][0-9][0-6][0-9]_[0-9]{4}[0-1][0-9][0-3][0-9]T[0-2][0-9][0-6][0-9][0-6][0-9]|MSIL2A_[0-9]{4}[0-1][0-9][0-3][0-9]T[0-2][0-9][0-6][0-9][0-6][0-9]_N...._R[0-9]{3}.*)\.SAFE</drb:nameMatch>
      </drb:signature>
   </owl:Class>

   <!-- ========================================= -->
   <!-- Metadata File (Level-2A)                  -->
   <!-- ========================================= -->

   <!-- Compliant with COMPACT -->
   <owl:Class rdf:about="&s2;userProductLevel2aMetadataFile">
      <rdfs:label xml:lang="en">User Product Level-2A: Metadata File</rdfs:label>
      <rdfs:comment xml:lang="en">
         The XML metadata file provided inside the S2 Level-2A User Product.
      </rdfs:comment>
      <rdfs:subClassOf rdf:resource="&drb;xml"/>
      <drb:signature rdf:parseType="Resource">
         <drb:parentIsSubClassTest>&s2;userProduct</drb:parentIsSubClassTest>
         <drb:nameMatch>(S2[AB]_...._MTD_(SAF|DMP)L2A_PDMC.*|MTD_MSIL2A.*)</drb:nameMatch>
      </drb:signature>
      <!-- This xsd is in the product, but in the repository too -->
      <drb:schemaLocation>
          xsd/int/esa/sentinel-2/S2_User_Product_Level-2A_Metadata.xsd
      </drb:schemaLocation>
   </owl:Class>

   <!-- ========================================= -->
   <!-- Metadata XSD (Level-2A)                   -->
   <!-- ========================================= -->

   <!-- Compliant with COMPACT -->
   <owl:Class rdf:about="&s2;userProductLevel2aMetadataXsd">
      <rdfs:label xml:lang="en">User Product Level-2A: Metadata XML Schema</rdfs:label>
      <rdfs:comment xml:lang="en">
         The XML schema describing the metadata file provided inside the S2
         Level-2A User Product.
      </rdfs:comment>
      <rdfs:subClassOf rdf:resource="&drb;item"/>
      <drb:signature rdf:parseType="Resource">
         <drb:parentClassTest>&s2;representationInformationFolder</drb:parentClassTest>
         <drb:nameMatch>S2_User_Product_Level-2A_Metadata.xsd</drb:nameMatch>
      </drb:signature>
   </owl:Class>

   <!-- ========================================= -->
   <!-- SAFE Level-2A Manifest File               -->
   <!-- ========================================= -->

   <!-- Compliant with COMPACT -->
   <owl:Class rdf:about="&s2;sentinel2Level2aSafeManifestFile">
      <rdfs:label xml:lang="en">Sentinel-2 Level-2A SAFE Manifest File</rdfs:label>
      <rdfs:comment xml:lang="en">
         XML file with fixed name L2A_Manifest.xml.
         There are two manifests in a Level-2A product:
         * the manifest.safe: comes from the Level-1C product used to generate
           the Level-2A product.
         * the L2A_Manifest.xml: the Level-2A product.'s manifest.         
      </rdfs:comment>
      <!--<rdfs:subClassOf rdf:resource="&drb;safe-manifest"/>-->
      <rdfs:subClassOf rdf:resource="&drb;xml"/>
      <drb:signature rdf:parseType="Resource">
         <drb:parentIsSubClassTest>&s2;item</drb:parentIsSubClassTest>
         <drb:nameTest>L2A_Manifest.xml</drb:nameTest>
      </drb:signature>
   </owl:Class>

   <!-- ========================================= -->
   <!-- Granule (Level-2A)                        -->
   <!-- ========================================= -->

   <!-- Compliant with COMPACT -->
   <owl:Class rdf:about="&s2;level2aGranule">
      <rdfs:label xml:lang="en">Level-2A Granule</rdfs:label>
      <rdfs:comment xml:lang="en">
         One of the granules composing the User Product Level-2A.
         A granule-folder corresponds to the Tile composing the product.
         The PDI Level-2A Granule/Tile consists of:
         1. Level-2A_Tile_Metadata_File (Tile Metadata): XML Main Metadata
             file (DIMAP mandatory file) containing the requested level of
             information and referring all the product elements describing the
             tile,
         2. IMG_DATA: folder containing image data files compressed using the
            JPEG2000 algorithm, one file per band.
         3. QI_DATA: folder containing OLQC XML reports of quality checks, mask
            files and PVI file;
         4. Inventory_Metadata.xml: file containing the metadata needed to
            inventory the PDI;
         5. manifest.safe: XML SAFE Manifest file;
         6. rep_info: folder containing the available XSD schemas that
            validate the PDI components.
         Note that the Inventory_Metadata.xml, manifest.safe and rep_info are
         available inside a Granule but they are removed when the PDI is
         included in the User Product.
      </rdfs:comment>
      <rdfs:subClassOf rdf:resource="&s2;granule"/>
      <drb:signature rdf:parseType="Resource">
         <drb:parentClassTest>&s2;granuleWrapper</drb:parentClassTest>
         <drb:nameMatch>(S2[AB]_...._MSI_L2A_TL.*_N[0-9]{2}\.[0-9]{2}|L2A_T....._A[0-9]{6}_[0-9]{4}[0-1][0-9][0-3][0-9]T[0-2][0-9][0-6][0-9][0-6][0-9])</drb:nameMatch>
      </drb:signature>
   </owl:Class>

   <!-- ========================================= -->
   <!-- Granule (Level-2A) / RXXm                 -->
   <!-- ========================================= -->

   <!-- Compliant with COMPACT -->
   <!-- ABSTRACT CLASS -->
   <!--
   <owl:Class rdf:about="&s2;level2aGranuleRXXm">
      <rdfs:label xml:lang="en">Level-2A Granule: Resolution XXm Folder</rdfs:label>
      <rdfs:comment xml:lang="en">
         Abstract class for R10m, R20m and R60m folders.
      </rdfs:comment>
      <rdfs:subClassOf rdf:resource="&drb;item"/>
      <drb:signature rdf:parseType="Resource">
         <drb:parentClassTest>&s2;imageFolder</drb:parentClassTest>
         <drb:nameMatch>R(10|20|60)m</drb:nameMatch>
      </drb:signature>
   </owl:Class>
   -->

   <!-- ========================================= -->
   <!-- Granule (Level-2A) / R10m                 -->
   <!-- ========================================= -->

   <!-- Compliant with COMPACT -->
   <!--
   <owl:Class rdf:about="&s2;level2aGranuleR10m">
      <rdfs:label xml:lang="en">Level-2A Granule: Resolution 10m Folder</rdfs:label>
      <rdfs:comment xml:lang="en">
         Image resolution = 10m.
      </rdfs:comment>
      <rdfs:subClassOf rdf:resource="&s2;level2aGranuleRXXm"/>
      <drb:signature rdf:parseType="Resource">
         <drb:parentClassTest>&s2;imageFolder</drb:parentClassTest>
         <drb:nameTest>R10m</drb:nameTest>
      </drb:signature>
   </owl:Class>
   -->

   <!-- ========================================= -->
   <!-- Granule (Level-2A) / R20m                 -->
   <!-- ========================================= -->

   <!-- Compliant with COMPACT -->
   <!--
   <owl:Class rdf:about="&s2;level2aGranuleR20m">
      <rdfs:label xml:lang="en">Level-2A Granule: Resolution 20m Folder</rdfs:label>
      <rdfs:comment xml:lang="en">
         Image resolution = 20m.
      </rdfs:comment>
      <rdfs:subClassOf rdf:resource="&s2;level2aGranuleRXXm"/>
      <drb:signature rdf:parseType="Resource">
         <drb:parentClassTest>&s2;imageFolder</drb:parentClassTest>
         <drb:nameTest>R20m</drb:nameTest>
      </drb:signature>
   </owl:Class>
   -->

   <!-- ========================================= -->
   <!-- Granule (Level-2A) / R60m                 -->
   <!-- ========================================= -->

   <!-- Compliant with COMPACT -->
   <!--
   <owl:Class rdf:about="&s2;level2aGranuleR60m">
      <rdfs:label xml:lang="en">Level-2A Granule: Resolution 60m Folder</rdfs:label>
      <rdfs:comment xml:lang="en">
         Image resolution = 60m.
      </rdfs:comment>
      <rdfs:subClassOf rdf:resource="&s2;level2aGranuleRXXm"/>
      <drb:signature rdf:parseType="Resource">
         <drb:parentClassTest>&s2;imageFolder</drb:parentClassTest>
         <drb:nameTest>R60m</drb:nameTest>
      </drb:signature>
   </owl:Class>
   -->

   <!-- ========================================= -->
   <!-- Tile Image File (Level-2A)                -->
   <!--    (Surface Reflectance Image)            -->
   <!-- ========================================= -->

   <!-- Compliant with COMPACT -->
   <owl:Class rdf:about="&s2;level2aTileImageFileSurfaceReflectanceImage">
      <rdfs:label xml:lang="en">Level-2A Tile Image File (Surface Reflectance Image)</rdfs:label>
      <rdfs:comment xml:lang="en">
         Surface Reflectance Image.
      </rdfs:comment>
      <rdfs:subClassOf rdf:resource="&jpeg2000;JPEG2000"/>
      <drb:signature rdf:parseType="Resource">
         <!--<drb:parentClassTest>&s2;level2aGranuleRXXm</drb:parentClassTest>-->
         <drb:nameMatch>(S2[AB]_...._MSI_L2A_.*|L2A_T....._[0-9]{4}[0-1][0-9][0-3][0-9]T[0-2][0-9][0-6][0-9][0-6][0-9])_B(01|02|03|04|05|06|07|08|09|10|11|12|8A)_(10|20|60)m\.(?i)jp2</drb:nameMatch>
      </drb:signature>
   </owl:Class>

   <!-- ========================================= -->
   <!-- Tile Image File (Level-2A)                -->
   <!--    (Resampled AOT Image)                  -->
   <!-- ========================================= -->

   <!-- Compliant with COMPACT -->
   <owl:Class rdf:about="&s2;level2aTileImageFileResampledAOTImage">
      <rdfs:label xml:lang="en">Level-2A Tile Image File (Resampled AOT Image)</rdfs:label>
      <rdfs:comment xml:lang="en">
         Resampled AOT Image.
      </rdfs:comment>
      <rdfs:subClassOf rdf:resource="&jpeg2000;JPEG2000"/>
      <drb:signature rdf:parseType="Resource">
         <!--<drb:parentClassTest>&s2;level2aGranuleRXXm</drb:parentClassTest>-->
         <drb:nameMatch>(S2[AB]_...._AOT_L2A_.*|L2A_T....._[0-9]{4}[0-1][0-9][0-3][0-9]T[0-2][0-9][0-6][0-9][0-6][0-9]_AOT)_(10|20|60)m\.(?i)jp2</drb:nameMatch>
      </drb:signature>
   </owl:Class>

   <!-- ========================================= -->
   <!-- Tile Image File (Level-2A)                -->
   <!--    (Water Vapour Image)                   -->
   <!-- ========================================= -->

   <!-- Compliant with COMPACT -->
   <owl:Class rdf:about="&s2;level2aTileImageFileWaterVapourImage">
      <rdfs:label xml:lang="en">Level-2A Tile Image File (Water Vapour Image)</rdfs:label>
      <rdfs:comment xml:lang="en">
         Water Vapour Image.
      </rdfs:comment>
      <rdfs:subClassOf rdf:resource="&jpeg2000;JPEG2000"/>
      <drb:signature rdf:parseType="Resource">
         <!--<drb:parentClassTest>&s2;level2aGranuleRXXm</drb:parentClassTest>-->
         <drb:nameMatch>(S2[AB]_...._WVP_L2A_.*|L2A_T....._[0-9]{4}[0-1][0-9][0-3][0-9]T[0-2][0-9][0-6][0-9][0-6][0-9]_WVP)_(10|20|60)m\.(?i)jp2</drb:nameMatch>
      </drb:signature>
   </owl:Class>

   <!-- ========================================= -->
   <!-- Tile Image File (Level-2A)                -->
   <!--    (Scene Classification Tile)            -->
   <!-- ========================================= -->

   <!-- Compliant with COMPACT -->
   <owl:Class rdf:about="&s2;level2aTileImageFileSceneClassificationTile">
      <rdfs:label xml:lang="en">Level-2A Tile Image File (Scene Classification Tile)</rdfs:label>
      <rdfs:comment xml:lang="en">
         Scene Classification Tile.
      </rdfs:comment>
      <rdfs:subClassOf rdf:resource="&jpeg2000;JPEG2000"/>
      <drb:signature rdf:parseType="Resource">
         <!--<drb:parentClassTest>&s2;level2aGranuleRXXm</drb:parentClassTest>-->
         <drb:nameMatch>(S2[AB]_...._SCL_L2A_.*|L2A_T....._[0-9]{4}[0-1][0-9][0-3][0-9]T[0-2][0-9][0-6][0-9][0-6][0-9]_SCL)_(10|20|60)m\.(?i)jp2</drb:nameMatch>
      </drb:signature>
   </owl:Class>

   <!-- ========================================= -->
   <!-- Tile Image File (Level-2A)                -->
   <!--    (True Color Image)                     -->
   <!-- ========================================= -->

   <!-- Compliant with COMPACT -->
   <owl:Class rdf:about="&s2;level2aTileImageFileTrueColorImage">
      <rdfs:label xml:lang="en">Level-2A Tile Image File (True Color Image)</rdfs:label>
      <rdfs:comment xml:lang="en">
         True Color Image.
      </rdfs:comment>
      <rdfs:subClassOf rdf:resource="&jpeg2000;JPEG2000"/>
      <drb:signature rdf:parseType="Resource">
         <!--<drb:parentClassTest>&s2;level2aGranuleRXXm</drb:parentClassTest>-->
         <drb:nameMatch>(S2[AB]_...._TCI_L2A_.*|L2A_T....._[0-9]{4}[0-1][0-9][0-3][0-9]T[0-2][0-9][0-6][0-9][0-6][0-9]_TCI)_(10|20|60)m\.(?i)jp2</drb:nameMatch>
      </drb:signature>
   </owl:Class>

   <!-- ========================================= -->
   <!-- Tile Metadata File (Level-2A)             -->
   <!-- ========================================= -->

   <!-- Compliant with COMPACT -->
   <owl:Class rdf:about="&s2;level2aGranuleMetadataFile">
      <rdfs:label xml:lang="en">Level-2A Granule Metadata File</rdfs:label>
      <rdfs:comment xml:lang="en">
         The XML metadata file provided inside each Level-2A tile.
      </rdfs:comment>
      <rdfs:subClassOf rdf:resource="&s2;granuleMetadataFile"/>
      <drb:signature rdf:parseType="Resource">
         <drb:parentClassTest>&s2;level2aGranule</drb:parentClassTest>
         <drb:xqueryTest>
            let $var := name(.)
            return
            if (fn:matches($var, "(S2[AB]_...._MTD_L2A_TL_.*|MTD_TL\.xml)") and
                ../../../*[matches(name(), "L2A_Manifest.xml")])
            then 1
            else 0
         </drb:xqueryTest>
      </drb:signature>
      <drb:schemaLocation>xsd/int/esa/sentinel-2/S2_PDI_Level-2A_Tile_Metadata.xsd</drb:schemaLocation>
   </owl:Class>

   <!-- ========================================= -->
   <!-- Tile Metadata XSD (Level-2A)              -->
   <!-- ========================================= -->

   <!-- Compliant with COMPACT -->
   <owl:Class rdf:about="&s2;level2aGranuleMetadataXsd">
      <rdfs:label xml:lang="en">Level-2A Granule Metadata XML Schema</rdfs:label>
      <rdfs:comment xml:lang="en">
         The XML schema describing the metadata file provided inside the S2
         Level-2A Granule.
      </rdfs:comment>
      <rdfs:subClassOf rdf:resource="&drb;item"/>
      <drb:signature rdf:parseType="Resource">
         <drb:parentClassTest>&s2;representationInformationFolder</drb:parentClassTest>
         <drb:nameMatch>S2_PDI_Level-2A_Tile_Metadata.xsd</drb:nameMatch>
      </drb:signature>
   </owl:Class>

   <!-- ========================================= -->
   <!-- Datastrip (Level-2A)                      -->
   <!-- ========================================= -->

   <!-- Compliant with COMPACT -->
   <owl:Class rdf:about="&s2;level2aDatastrip">
      <rdfs:label xml:lang="en">Level-2A Datastrip</rdfs:label>
      <rdfs:comment xml:lang="en">
         One of the datastrips for User Product Level-2A.
         The PDI Level 2A DataStrip consists of:
         1. DataStrip_Metadata_File: XML Main Metadata file (DIMAP mandatory
            file) containing the requested level of information and referring all
            the product elements describing the DataStrip.
         2. QI_DATA: folder containing XML reports providing Quality control
            checks information.
         4. Inventory_Metadata.xml: file containing the metadata needed to
            inventory the PDI;
         5. manifest.safe: XML SAFE Manifest file;
         6. rep_info: folder containing the available XSD schemas that
            validate the PDI components.
         Note that the Inventory_Metadata.xml, manifest.safe and rep_info are
         available inside a Datastrip but they are removed when the PDI is
         included in the User Product.
      </rdfs:comment>
      <rdfs:subClassOf rdf:resource="&s2;datastrip"/>
      <drb:signature rdf:parseType="Resource">
         <drb:parentClassTest>&s2;datastripWrapper</drb:parentClassTest>
         <drb:xqueryTest>
            let $var := name(.)
            return
            if (fn:matches($var, "(S2[AB]_...._MSI_L2A_DS.*_N[0-9]{2}\.[0-9]{2}|DS_...._[0-9]{4}[0-1][0-9][0-3][0-9]T[0-2][0-9][0-6][0-9][0-6][0-9]_S[0-9]{4}[0-1][0-9][0-3][0-9]T[0-2][0-9][0-6][0-9][0-6][0-9])") and
                ../../*[matches(name(), "L2A_Manifest.xml")])
            then 1
            else 0
         </drb:xqueryTest>
      </drb:signature>
   </owl:Class>

   <!-- ========================================= -->
   <!-- Datastrip Metadata File (Level-2A)        -->
   <!-- ========================================= -->

   <!-- Compliant with COMPACT -->
   <owl:Class rdf:about="&s2;level2aDatastripMetadataFile">
      <rdfs:label xml:lang="en">Level-2A Datastrip Metadata File</rdfs:label>
      <rdfs:comment xml:lang="en">
         XML Metadata file (DIMAP mandatory file) containing the requested
         level of information and referring all the product elements describing
         the datastrip.
      </rdfs:comment>
      <rdfs:subClassOf rdf:resource="&s2;datastripMetadataFile"/>
      <drb:signature rdf:parseType="Resource">
         <drb:parentClassTest>&s2;level2aDatastrip</drb:parentClassTest>
         <drb:xqueryTest>
            let $var := name(.)
            return
            if (fn:matches($var, "(S2[AB]_...._MTD_L2A_DS_.*|MTD_DS.*)") and
                ../../../*[matches(name(), "L2A_Manifest.xml")])
            then 1
            else 0
         </drb:xqueryTest>
      </drb:signature>
      <drb:schemaLocation>xsd/int/esa/sentinel-2/S2_PDI_Level-2A_Datastrip_Metadata.xsd</drb:schemaLocation>
   </owl:Class>

   <!-- ========================================= -->
   <!-- Datastrip Metadata XSD (Level-2A)         -->
   <!-- ========================================= -->

   <!-- Compliant with COMPACT -->
   <owl:Class rdf:about="&s2;level2aDatastripMetadataXsd">
      <rdfs:label xml:lang="en">Level-2A Datastrip Metadata XML Schema</rdfs:label>
      <rdfs:comment xml:lang="en">
         The XML schema describing the metadata file provided inside the S2
         Level-2A Datastrip.
      </rdfs:comment>
      <rdfs:subClassOf rdf:resource="&drb;item"/>
      <drb:signature rdf:parseType="Resource">
         <drb:parentClassTest>&s2;representationInformationFolder</drb:parentClassTest>
         <drb:nameMatch>S2_PDI_Level-2A_Datastrip_Metadata.xsd</drb:nameMatch>
      </drb:signature>
   </owl:Class>

   <!-- ========================================= -->
   <!-- Under QI_DATA Folder:                     -->
   <!-- L2A Quality Mask:                         -->
   <!-- Confidence Cloud Mask File                -->
   <!-- ========================================= -->

   <!-- Compliant with COMPACT -->
   <owl:Class rdf:about="&s2;level2aTileImageFileConfidenceCloudMaskFile">
      <rdfs:label xml:lang="en">Level-2A Quality Mask (Confidence Cloud Mask File)</rdfs:label>
      <rdfs:comment xml:lang="en">
         Level-2A Quality Mask (Confidence Cloud Mask File).
      </rdfs:comment>
      <rdfs:subClassOf rdf:resource="&jpeg2000;JPEG2000"/>
      <drb:signature rdf:parseType="Resource">
         <drb:parentClassTest>&s2;qualityControlFolder</drb:parentClassTest>
         <drb:nameMatch>(S2[AB]_...._CLD_L2A_.*|L2A_T....._[0-9]{4}[0-1][0-9][0-3][0-9]T[0-2][0-9][0-6][0-9][0-6][0-9]_CLD)_(10|20|60)m\.(?i)jp2</drb:nameMatch>
      </drb:signature>
   </owl:Class>

   <!-- ========================================= -->
   <!-- Under QI_DATA Folder:                     -->
   <!-- L2A Quality Mask:                         -->
   <!-- Confidence Snow Mask File                 -->
   <!-- ========================================= -->

   <!-- Compliant with COMPACT -->
   <owl:Class rdf:about="&s2;level2aTileImageFileConfidenceSnowMaskFile">
      <rdfs:label xml:lang="en">Level-2A Quality Mask (Confidence Snow Mask File)</rdfs:label>
      <rdfs:comment xml:lang="en">
         Level-2A Quality Mask (Confidence Snow Mask File).
      </rdfs:comment>
      <rdfs:subClassOf rdf:resource="&jpeg2000;JPEG2000"/>
      <drb:signature rdf:parseType="Resource">
         <drb:parentClassTest>&s2;qualityControlFolder</drb:parentClassTest>
         <drb:nameMatch>(S2[AB]_...._SNW_L2A_.*|L2A_T....._[0-9]{4}[0-1][0-9][0-3][0-9]T[0-2][0-9][0-6][0-9][0-6][0-9]_SNW)_(10|20|60)m\.(?i)jp2</drb:nameMatch>
      </drb:signature>
   </owl:Class>

   <!-- ========================================= -->
   <!-- Under QI_DATA Folder:                     -->
   <!-- PVI Tile Preview Image                    -->
   <!-- ========================================= -->

   <!-- Compliant with COMPACT -->
   <owl:Class rdf:about="&s2;level2aTileImageFilePviTilePreviewImage">
      <rdfs:label xml:lang="en">PVI Tile Preview Image</rdfs:label>
      <rdfs:comment xml:lang="en">
         PVI Tile Preview Image.
      </rdfs:comment>
      <rdfs:subClassOf rdf:resource="&jpeg2000;JPEG2000"/>
      <drb:signature rdf:parseType="Resource">
         <drb:parentClassTest>&s2;qualityControlFolder</drb:parentClassTest>
         <drb:nameMatch>(S2[AB]_...._PVI_L2A_.*|L2A_T....._[0-9]{4}[0-1][0-9][0-3][0-9]T[0-2][0-9][0-6][0-9][0-6][0-9]_PVI)_(10|20|60)m\.(?i)jp2</drb:nameMatch>
      </drb:signature>
   </owl:Class>

</rdf:RDF>
