<?xml version="1.0" encoding="ISO-8859-1" standalone="yes"?>

<!DOCTYPE rdf:RDF [
   <!ENTITY rdf "http://www.w3.org/1999/02/22-rdf-syntax-ns#">
   <!ENTITY rdfs "http://www.w3.org/2000/01/rdf-schema#">
   <!ENTITY owl "http://www.w3.org/2002/07/owl#">
   <!ENTITY s2   "http://www.esa.int/s2#">
   <!ENTITY drb "http://www.gael.fr/drb#">
   <!ENTITY jpeg2000 "http://www.gael.fr/drb/jpeg2000#">
]>

<rdf:RDF xmlns:owl="&owl;"
         xmlns:rdf="&rdf;"
         xmlns:rdfs="&rdfs;"
         xmlns:drb="&drb;"
         xmlns:jpeg2000="&jpeg2000;"
         xmlns:s2="&s2;"
         xml:base="&s2;">

<!--
* Data Hub Service (DHuS) - For Space data distribution.
* Copyright (C) 2013,2014,2015,2016 GAEL Systems
*
* This file is part of DHuS software sources.
*
* This program is free software: you can redistribute it and/or modify
* it under the terms of the GNU Affero General Public License as
* published by the Free Software Foundation, either version 3 of the
* License, or (at your option) any later version.
*
* This program is distributed in the hope that it will be useful,
* but WITHOUT ANY WARRANTY; without even the implied warranty of
* MERCHANTABILITY or FITNESS FOR A PARTICULAR PURPOSE. See the
* GNU Affero General Public License for more details.
*
* You should have received a copy of the GNU Affero General Public License
* along with this program. If not, see <http://www.gnu.org/licenses/>.
-->

   <owl:Ontology rdf:about="&s2;">
      <rdfs:label xml:lang="en">Sentinel-2 Level-0 Ontology</rdfs:label>
   </owl:Ontology>

   <!-- ========================================= -->
   <!-- User Level-0 Product                      -->
   <!-- ========================================= -->

   <!-- WARN ID changed
        <owl:Class rdf:about="&s2;userLevel0Product"> -->
   <!-- Back to previous ID for compatibility
   <owl:Class rdf:about="&s2;userProductLevel0">-->
   <owl:Class rdf:about="&s2;userLevel0Product">
      <rdfs:label xml:lang="en">Sentinel-2 User Product Level-0</rdfs:label>
      <rdfs:comment xml:lang="en">
         Level-0 product is generated from the Sentinel-2 instrument and 
         ancillary telemetries. It contains raw data after restoration of the 
         chronological data sequence at full space/time resolution with all 
         auxiliary and ancillary information to be used in subsequent
         processing. In fact the Level-0 product contains all the information
         required to generate the Level-1 (and upper) product levels. The 
         Level-0 consolidation processing stores the Quick Look image in the L0
         DataStrip PDI. Reprocessing is from archived consolidated L0 which
         include QL image to get Level 1 products.
         One Level-0 product refers always to one Datatake; it can cover the 
         full Datatake or an its extract. It may refer to one or several
         DataStrips from the same Datatake.
         The Level-0 User product consists of: 
         1. Product_Metadata_File: This is the mandatory XML main metadata file
         (DIMAP) containing the requested level of information and referring
         all the product elements.
         2. manifest.safe: this is the SAFE metadata file (optional). It is
         included in the product only if the user requests a SAFE product as
         output format (according to a specific download option).
         3. GRANULE: folder containing all granules composing the product
         (Image Data). The Image Data files inside each Granule are provided as
         a set of 13 binary files, one image file per band corresponding to a
         given detector.
         4. DATASTRIP: folder containing the DataStrip composing the product
         linked to the selected granules.
         5. AUX_DATA: folder containing, if requested by the user (download
         option), the GIPP files and IERS Bulletins used for the Level-0 User
         Product production. All Level-0 auxiliary data are referenced in the
         product metadata file.
         6. ANC_DATA: folder containing the Satellite Ancillary Data (SAD)
         needed for the processing (GPS data, attitude data, etc.). The SAD are
         always provided as a set of unitary Raw Data files each matching a
         single packet type. Those files are provided on the same temporal
         extent of the SAD embedded in the last Datastrip selected to be
         included in the product.
         7. rep_info: folder containing the XSD schema provided inside the 
         product. This folder is optional. It will be included in the final
         product if the user select the SAFE format as output format.
         8. Browse_Image: PNG file consisting of an image limited to 3
         visible-bands in ground geometry at 320m resolution. This file,
         provided if required by the user (download option), gives an overview
         of the product (sub-sampled) mainly for image data browsing and
         selection purposes.
         9. INSPIRE: XML INSPIRE metadata file.
         10. HTML: folder containing an HTML product presentation file
         (UserProduct_index.html) and the corresponding stylesheet
         (UserProduct_index.xsl).
         Note: The number of the Granules available within a L0 product is
         variable and driven by the active detectors list specified at
         Datastrip level (ACTIVE_DETECTOR metadata). The list of the active
         detectors depends on the MSI acquisition mode (compression by-passed
         or not).
         Compression mode is reported in the MSI packet by the MODOP field.
         In the nominal products the compression is enabled and all detectors
         are available; in case of calibration products the compression is
         by-passed and only a subset of detectors are active and therefore
         available.
      </rdfs:comment>
       <rdfs:subClassOf rdf:resource="&s2;userProduct"/>
      <drb:signature rdf:parseType="Resource">
         <drb:nameMatch>S2[AB]_...._PRD_MSIL0P_PDMC_[0-9]{4}[0-1][0-9][0-3][0-9]T[0-2][0-9][0-6][0-9][0-6][0-9]_R[0-9]{3}_V[0-9]{4}[0-1][0-9][0-3][0-9]T[0-2][0-9][0-6][0-9][0-6][0-9]_[0-9]{4}[0-1][0-9][0-3][0-9]T[0-2][0-9][0-6][0-9][0-6][0-9]\.SAFE</drb:nameMatch>
      </drb:signature>
   </owl:Class>

   <!-- ========================================= -->
   <!-- Metadata File (Level-0)                   -->
   <!-- ========================================= -->

   <owl:Class rdf:about="&s2;userProductLevel0MetadataFile">
      <rdfs:label xml:lang="en">Sentinel-2 User Product Level-0: Metadata File</rdfs:label>
      <rdfs:comment xml:lang="en">
         The XML metadata file provided inside the S2 Level-0 User Product.
      </rdfs:comment>
      <rdfs:subClassOf rdf:resource="&drb;xml"/>
      <drb:signature rdf:parseType="Resource">
         <drb:nameMatch>S2[AB]_...._MTD_(SAF|DMP)L0P_PDMC.*</drb:nameMatch>
         <drb:parentIsSubClassTest>&s2;userProduct</drb:parentIsSubClassTest>
      </drb:signature>
      <!-- This xsd is in the product, but in the repository too -->
      <drb:schemaLocation>
          xsd/int/esa/sentinel-2/S2_User_Product_Level-0_Metadata.xsd
      </drb:schemaLocation>
   </owl:Class>

   <!-- ========================================= -->
   <!-- Metadata XSD (Level-0)                    -->
   <!-- ========================================= -->

   <owl:Class rdf:about="&s2;userProductLevel0MetadataXsd">
      <rdfs:label xml:lang="en">Sentinel-2 User Product Level-0: Metadata XML Schema</rdfs:label>
      <rdfs:comment xml:lang="en">
         The XML schema describing the metadata file provided inside the S2
         Level-0 User Product.
      </rdfs:comment>
      <rdfs:subClassOf rdf:resource="&drb;item"/>
      <drb:signature rdf:parseType="Resource">
         <drb:nameMatch>S2_User_Product_Level-0_Metadata.xsd</drb:nameMatch>
         <drb:parentClassTest>&s2;representationInformationFolder</drb:parentClassTest>
      </drb:signature>
   </owl:Class>

   <!-- ========================================= -->
   <!-- Granule (Level-0)                         -->
   <!-- ========================================= -->

   <!-- WARN ID changed
       <owl:Class rdf:about="&s2;pdi_level_0_granule_container"> -->
   <owl:Class rdf:about="&s2;level0Granule">
      <rdfs:label xml:lang="en">Sentinel-2 Level-0 Granule</rdfs:label>
      <rdfs:comment xml:lang="en">
         One of the granules composing the User Product Level-0.
         The PDI Level-0 granule consists of:
         1. Level-0_Granule_Metadata_File: XML metadata file containing the
            requested level of information and referring all the product
            elements composing the Granule;
         2. IMG_DATA: folder containing the mission data corresponding to one
            on-board scene for one detector and all spectral bands. The image
            data are provided as a set of 13 binary files, one for each spectral
            band, including all corresponding Image Source Packets (ISP) in the
            observation chronological sequence. The ISPs include their
            corresponding source packet annotations as a pre-pended header of
            each source packet;
         3. QI_DATA: folder containing XML reports about Geometric quality,
            Image content quality, Quality control checks information;
         4. Inventory_Metadata.xml: file containing the metadata needed to
            inventory the PDI;
         5. manifest.safe: XML SAFE Manifest file;
         6. rep_info: folder containing the available XSD schemas that validate
            the PDI components.
         Note that the Inventory_Metadata.xml, manifest.safe and rep_info are
         available inside a Granule but they are removed when the PDI is
         included in the User Product.
      </rdfs:comment>
      <rdfs:subClassOf rdf:resource="&s2;granule"/>
      <drb:signature rdf:parseType="Resource">
         <drb:nameMatch>S2[AB]_...._MSI_L0__GR.*_N[0-9]{2}\.[0-9]{2}</drb:nameMatch>
         <!--
         <drb:parentClassTest>&s2;granuleWrapper</drb:parentClassTest>
         -->
      </drb:signature>
   </owl:Class>

   <!-- ========================================= -->
   <!-- Granule ISP File (Level-0)                -->
   <!-- ========================================= -->

   <!-- WARN ID changed
        <owl:Class rdf:about="&s2;pdi_isp"> -->
   <owl:Class rdf:about="&s2;level0IspFile">
      <rdfs:label xml:lang="en">Sentinel-2 Level-0 ISP File</rdfs:label>
      <rdfs:comment xml:lang="en">
         Level 0 CCSDS formatted source packets data. One file per band.
      </rdfs:comment>
      <rdfs:subClassOf rdf:resource="&s2;item"/>
      <drb:signature rdf:parseType="Resource">
         <drb:nameMatch>S2[AB]_...._MSI_L0_.*_B(01|02|03|04|05|06|07|08|09|10|11|12|8A)\.(?i)bin</drb:nameMatch>
         <drb:parentClassTest>&s2;imageFolder</drb:parentClassTest>
      </drb:signature>
   </owl:Class>

   <!-- ========================================= -->
   <!-- Granule Metadata File (Level-0)           -->
   <!-- ========================================= -->

   <!-- WARN ID changed
        <owl:Class rdf:about="&s2;pdi_level_0_granule_metadata"> -->
   <owl:Class rdf:about="&s2;level0GranuleMetadataFile">
      <rdfs:label xml:lang="en">Sentinel-2 Level-0 Granule Metadata File</rdfs:label>
      <rdfs:comment xml:lang="en">
         XML metadata file containing the requested level of information and
         referring all the product elements composing the Granule.
      </rdfs:comment>
      <rdfs:subClassOf rdf:resource="&s2;granuleMetadataFile"/>
      <drb:signature rdf:parseType="Resource">
         <drb:parentClassTest>&s2;level0Granule</drb:parentClassTest>
         <drb:nameMatch>S2[AB]_...._MTD_L0__GR_.*</drb:nameMatch>
      </drb:signature>
      <drb:schemaLocation>xsd/int/esa/sentinel-2/S2_PDI_Level-0_Granule_Metadata.xsd</drb:schemaLocation>
   </owl:Class>

   <!-- ========================================= -->
   <!-- Datastrip (Level-0)                       -->
   <!-- ========================================= -->

   <!-- WARN ID changed
        <owl:Class rdf:about="&s2;pdi_level_0_datastrip_container"> -->
   <owl:Class rdf:about="&s2;level0Datastrip">
      <rdfs:label xml:lang="en">Sentinel-2 Level-0 Datastrip</rdfs:label>
      <rdfs:comment xml:lang="en">
         One of the datastrips for User Product Level-0.
         The PDI Level-0 Datastrip consists of:
         1. Datastrip_Metadata_File: XML metadata file containing the requested
            level of information and referring all the product elements
            composing the Datastrip;
         2. QI_DATA: folder containing the preliminary QuickLook files in JP2
            format and XML reports providing Quality control check results;
         3. ANC_DATA: folder containing SAD raw data provided on temporal
            extent of the full Datatake if the Datastrip is the last one in a
            given Datatake, otherwise the SAD coverage is from the start of the
            Datatake (to which the Datastrip belongs to) to the stop of the
            Datastrip itself. SAD data are provided as a set of unitary Raw Data
            files each matching a single packet type;
         4. Inventory_Metadata.xml: file containing the metadata needed to
            inventory the PDI;
         5. manifest.safe: XML SAFE Manifest file;
         6. rep_info: folder containing the available XSD schema that validate
            the PDI components
         Note that the ANC_DATA, Inventory_Metadata.xml, manifest.safe and
         rep_info are available inside a Datastrip but they are removed when
         the PDI is included in the User Product.
      </rdfs:comment>
      <rdfs:subClassOf rdf:resource="&s2;datastrip"/>
      <drb:signature rdf:parseType="Resource">
         <drb:nameMatch>S2[AB]_...._MSI_L0__DS.*_N[0-9]{2}\.[0-9]{2}</drb:nameMatch>
         <!--
         <drb:parentClassTest>&s2;datastripWrapper</drb:parentClassTest>
         -->
      </drb:signature>
   </owl:Class>

   <!-- ========================================= -->
   <!-- Datastrip QuickLook File (Level-0)        -->
   <!-- ========================================= -->

   <owl:Class rdf:about="&s2;level0QuicklookFile">
      <rdfs:label xml:lang="en">Sentinel-2 Level-0 QuickLook File</rdfs:label>
      <rdfs:comment xml:lang="en">
         Preliminary Quick Look files (JPEG2000 format). There is up to 5 files.
         The number of files could be potentially less than 5 in degraded cases.
      </rdfs:comment>
      <rdfs:subClassOf rdf:resource="&jpeg2000;JPEG2000"/>
      <drb:signature rdf:parseType="Resource">
         <drb:nameMatch>S2[AB]_...._QLK_L0__DS.*_B(01|02|03|04|05|06|07|08|09|10|11|12|8A)\.(?i)jp2</drb:nameMatch>
         <drb:parentClassTest>&s2;qualityControlFolder</drb:parentClassTest>
      </drb:signature>
   </owl:Class>

   <!-- ========================================= -->
   <!-- Datastrip Metadata File (Level-0)         -->
   <!-- ========================================= -->

   <!-- WARN ID changed
        <owl:Class rdf:about="&s2;pdi_level_0_datastrip_metadata"> -->
   <owl:Class rdf:about="&s2;level0DatastripMetadataFile">
      <rdfs:label xml:lang="en">Sentinel-2 Level-0 Datastrip Metadata File</rdfs:label>
      <rdfs:comment xml:lang="en">
         XML Metadata file (DIMAP mandatory file) containing the requested level
         of information and referring all the product elements describing the
         datastrip.
      </rdfs:comment>
      <rdfs:subClassOf rdf:resource="&s2;datastripMetadataFile"/>
      <drb:signature rdf:parseType="Resource">
         <drb:nameMatch>S2[AB]_...._MTD_L0__DS_.*</drb:nameMatch>
         <drb:parentClassTest>&s2;level0Datastrip</drb:parentClassTest>
      </drb:signature>
      <drb:schemaLocation>xsd/int/esa/sentinel-2/S2_PDI_Level-0_Datastrip_Metadata.xsd</drb:schemaLocation>
   </owl:Class>

   <!-- ========================================= -->
   <!-- Ancillary Data                            -->
   <!-- ========================================= -->

   <!-- WARN ID changed
        <owl:Class rdf:about="&s2;pdi_anc_folder"> -->
   <owl:Class rdf:about="&s2;ancillaryDataFolder">
      <rdfs:label xml:lang="en">Sentinel-2 Ancillary Data Folder</rdfs:label>
      <rdfs:comment xml:lang="en">
         PDI Case:
         Folder containing SAD raw data as received from the DFEP. Note that
         this folder is provided only inside a Level-0 Datastrip PDI.
         User product case:
         Folder containing the Satellite Ancillary Data (SAD) needed for the
         processing (GPS data, attitude data, etc.). The SAD are always provided
         as a set of unitary Raw Data files each matching a single packet type.
         Those files are provided on the same temporal extent of the SAD
         embedded in the last Datastrip selected to be included in the product.
         Raw Satellite Ancillary Data (SAD) are provided inside the Level-0
         User Product within the ANC_DATA folder. SAD data (DPC and DFEP
         annotated source packets, cf. §4.6.2.1) are splitted in binary files
         divided by PRID and SID (cf. Table 3-9). In order to have the maximum
         coverage of the raw SAD in the L0 User Product, the latest SAD related
         to the downlink time will be embeded in the product.
         The decoded SAD, useful for further processing are provided at
         Datastrip level through the Datastrip metadata file. In particular,
         these data allow computing the associated geometric model and include:
         * Time Correlation Data (sampled at 1Hz);
         * Imaging orbit number;
         * Ephemeris data;
         * Attitudes data (sampled at 10Hz);
         * Thermal data.
      </rdfs:comment>
      <rdfs:subClassOf rdf:resource="&drb;item"/>
      <drb:signature rdf:parseType="Resource">
         <drb:parentIsSubClassTest>&s2;pdi_container</drb:parentIsSubClassTest>
         <drb:nameTest>ANC_DATA</drb:nameTest>
      </drb:signature>
   </owl:Class>

   <!-- =================================================================== -->
   <!-- ZIP that contains Tar Granules and Datastrip                        -->
   <!-- =================================================================== -->

   <!--
   S2B_OPER_MSI_L0__LT_SGS__20191014T075559_S20191014T050726_N02.08.zip
      S2B_OPER_MSI_L0__LT_SGS__20191014T075559_S20191014T050726_N02.08/
         S2B_OPER_MSI_L0__DS_SGS__20191014T075559_S20191014T050726_N02.08.tar
         S2B_OPER_MSI_L0__GR_SGS__20191014T075559_S20191014T050726_D01_N02.08.tar
         S2B_OPER_MSI_L0__GR_SGS__20191014T075559_S20191014T050726_D02_N02.08.tar
         S2B_OPER_MSI_L0__GR_SGS__20191014T075559_S20191014T050726_D03_N02.08.tar
         etc.
   -->

   <owl:Class rdf:about="&s2;level0GranuleDatastripZip">
      <rdfs:label xml:lang="en">Sentinel-2 Level-0 Granules and Datastrip ZIP package</rdfs:label>
      <rdfs:comment xml:lang="en">
         The ZIP package contains a collection of granules with their related
         datastrip.
      </rdfs:comment>
      <rdfs:subClassOf rdf:resource="&s2;itemZipped"/>
      <drb:signature rdf:parseType="Resource">
         <drb:nameMatch>S2[AB]_...._MSI_L0__LT.*_N[0-9]{2}\.[0-9]{2}\.zip</drb:nameMatch>
      </drb:signature>
   </owl:Class>

   <!-- =================================================================== -->
   <!-- TAR Granule and Datastrip                                           -->
   <!-- =================================================================== -->

   <!-- ========================================= -->
   <!-- Tar Granule (Level-0)                     -->
   <!-- ========================================= -->

   <owl:Class rdf:about="&s2;level0GranuleTar">
      <rdfs:label xml:lang="en">Sentinel-2 Level-0 Tar Granule</rdfs:label>
      <rdfs:comment xml:lang="en">
         The PDI Level-0 Tar granule contains a PDI Level-0 granule, which
         consists of:
         1. Level-0_Granule_Metadata_File: XML metadata file containing the
            requested level of information and referring all the product
            elements composing the Granule;
         2. IMG_DATA: folder containing the mission data corresponding to one
            on-board scene for one detector and all spectral bands. The image
            data are provided as a set of 13 binary files, one for each spectral
            band, including all corresponding Image Source Packets (ISP) in the
            observation chronological sequence. The ISPs include their
            corresponding source packet annotations as a pre-pended header of
            each source packet;
         3. QI_DATA: folder containing XML reports about Geometric quality,
            Image content quality, Quality control checks information;
         4. Inventory_Metadata.xml: file containing the metadata needed to
            inventory the PDI;
         5. manifest.safe: XML SAFE Manifest file;
         6. rep_info: folder containing the available XSD schemas that validate
            the PDI components.
         Note that the Inventory_Metadata.xml, manifest.safe and rep_info are
         available inside a Granule but they are removed when the PDI is
         included in the User Product.
      </rdfs:comment>
      <rdfs:subClassOf rdf:resource="&s2;item"/>
      <rdfs:subClassOf rdf:resource="&drb;tar"/>
      <drb:signature rdf:parseType="Resource">
         <drb:nameMatch>S2[AB]_...._MSI_L0__GR.*_N[0-9]{2}\.[0-9]{2}\.tar</drb:nameMatch>
      </drb:signature>
   </owl:Class>

   <!-- ========================================= -->
   <!-- Tar Datastrip (Level-0)                   -->
   <!-- ========================================= -->

   <owl:Class rdf:about="&s2;level0DatastripTar">
      <rdfs:label xml:lang="en">Sentinel-2 Level-0 Tar Datastrip</rdfs:label>
      <rdfs:comment xml:lang="en">
         The PDI Level-0 Tar Datastrip contains a PDI Level-0 Datastrip, which
         consists of:
         1. Datastrip_Metadata_File: XML metadata file containing the requested
            level of information and referring all the product elements
            composing the Datastrip;
         2. QI_DATA: folder containing the preliminary QuickLook files in JP2
            format and XML reports providing Quality control check results;
         3. ANC_DATA: folder containing SAD raw data provided on temporal
            extent of the full Datatake if the Datastrip is the last one in a
            given Datatake, otherwise the SAD coverage is from the start of the
            Datatake (to which the Datastrip belongs to) to the stop of the
            Datastrip itself. SAD data are provided as a set of unitary Raw Data
            files each matching a single packet type;
         4. Inventory_Metadata.xml: file containing the metadata needed to
            inventory the PDI;
         5. manifest.safe: XML SAFE Manifest file;
         6. rep_info: folder containing the available XSD schema that validate
            the PDI components
         Note that the ANC_DATA, Inventory_Metadata.xml, manifest.safe and
         rep_info are available inside a Datastrip but they are removed when
         the PDI is included in the User Product.
      </rdfs:comment>
      <rdfs:subClassOf rdf:resource="&s2;item"/>
      <rdfs:subClassOf rdf:resource="&drb;tar"/>
      <drb:signature rdf:parseType="Resource">
         <drb:nameMatch>S2[AB]_...._MSI_L0__DS.*_N[0-9]{2}\.[0-9]{2}\.tar</drb:nameMatch>
      </drb:signature>
   </owl:Class>

   <!-- =================================================================== -->
   <!-- TAR HKTM (Level-0)                                                  -->
   <!-- =================================================================== -->

   <owl:Class rdf:about="&s2;level0HktmTar">
      <rdfs:label xml:lang="en">Sentinel-2 Level-0 Tar HKTM</rdfs:label>
      <rdfs:comment xml:lang="en">
         House Keeping Telemetry (HKTM) PDI are routed to FOS after their
         generation at CGS.
         Spacecraft housekeeping telemetry is part of the ancillary data and is
         regularly downlinked to ground stations (every orbit). Raw VCDUs are
         provided with DFEP annotation as a separated file.
         The HKTM PDI is formatted according to SAFE Specifications.
         It is defined as a tar file. It consists of:
         1. Measurement Data file (Binary File): binary encoded file containing
         the stream of HKTM Transfer Frames TFs.
         2. DFEP Annotation file (Binary File): binary file composed by one
         record for each HKTM TF, containing the TF annotations computed by the
         DFEP.
         3. manifest.safe (XML File): manifest file that includes metadata
         information describing the overall context where the HKTM data are
         generated (mission, product history, timing, orbit, etc.) and providing
         information regarding the content and structure of the product, through
         references to the other components present in the product.
         4. rep_info (Folder): folder containing the XSD schemas related to the
         Measurement Data and DFEP Annotation.
      </rdfs:comment>
      <rdfs:subClassOf rdf:resource="&s2;item"/>
      <rdfs:subClassOf rdf:resource="&drb;tar"/>
      <drb:signature rdf:parseType="Resource">
         <drb:nameMatch>S2[AB]_...._PRD_HKTM___[0-9]{8}T[0-9]{6}_[0-9]{8}T[0-9]{6}_[0-9]{4}\.tar</drb:nameMatch>
      </drb:signature>
   </owl:Class>

   <!-- =================================================================== -->
   <!-- TAR SAD PDI (AUX)                                                   -->
   <!-- =================================================================== -->

   <owl:Class rdf:about="&s2;pdiSadTar">
      <rdfs:label xml:lang="en">Sentinel-2 Auxiliary Tar SAD PDI</rdfs:label>
      <rdfs:comment xml:lang="en">
      RAW Satellite Ancillary Data (SAD) data are systematically downlinked to
      ground stations at the end of each downlink as source packets provided
      with their DFEP annotation.
      Each SAD packets include their corresponding source packet binary
      annotations as a pre-pended header. A source packet header consists
      (according to this order) in:
      * DPC annotation computed during the L0 processing DPC annotation;
      * DFEP annotation as received from the DFEP.
      SAD data (used mainly by the POD) are stored as a PDI.
      A SAD PDI consists in a single tar file containing a set of unitary Raw
      SAD files each matching a single packet type. Those files cover the
      temporal extent of the full orbit.
      </rdfs:comment>
      <rdfs:subClassOf rdf:resource="&s2;item"/>
      <rdfs:subClassOf rdf:resource="&drb;tar"/>
      <drb:signature rdf:parseType="Resource">
         <drb:nameMatch>S2[AB]_...._AUX_SADATA_...._[0-9]{8}T[0-9]{6}_V[0-9]{8}T[0-9]{6}_[0-9]{8}T[0-9]{6}_......._.._..\.tar</drb:nameMatch>
      </drb:signature>
   </owl:Class>

   <!-- =================================================================== -->
   <!-- GIPP (AUX)                                                          -->
   <!-- =================================================================== -->

   <!-- ========================================= -->
   <!-- GIPP TGZ                                  -->
   <!-- ========================================= -->

   <!-- Example
   S2A_OPER_GIP_ATMIMA_MPC__20150605T094744_V20150622T000000_21000101T000000_B00.TGZ
   -->
   <owl:Class rdf:about="&s2;gippTgz">
      <rdfs:label xml:lang="en">Sentinel-2 Auxiliary GIPP Tar/Gz</rdfs:label>
      <rdfs:comment xml:lang="en">
      TODO
      </rdfs:comment>
      <rdfs:subClassOf rdf:resource="&s2;item"/>
      <rdfs:subClassOf rdf:resource="&drb;tgz"/>
      <drb:signature rdf:parseType="Resource">
         <drb:nameMatch>S2[AB]_...._GIP_......_...._[0-9]{8}T[0-9]{6}_V[0-9]{8}T[0-9]{6}_[0-9]{8}T[0-9]{6}_...\.TGZ</drb:nameMatch>
      </drb:signature>
   </owl:Class>

   <!-- ========================================= -->
   <!-- GIPP TAR                                  -->
   <!-- ========================================= -->

   <!-- Example
   S2A_OPER_GIP_ATMIMA_MPC__20150605T094744_V20150622T000000_21000101T000000_B00.tar
   -->
   <owl:Class rdf:about="&s2;gippTar">
      <rdfs:label xml:lang="en">Sentinel-2 Auxiliary GIPP Tar</rdfs:label>
      <rdfs:comment xml:lang="en">
      TODO
      </rdfs:comment>
      <rdfs:subClassOf rdf:resource="&s2;item"/>
      <rdfs:subClassOf rdf:resource="&drb;tar"/>
      <drb:signature rdf:parseType="Resource">
         <drb:nameMatch>(?i)S2[AB]_...._GIP_......_...._[0-9]{8}T[0-9]{6}_V[0-9]{8}T[0-9]{6}_[0-9]{8}T[0-9]{6}_...\.tar</drb:nameMatch>
      </drb:signature>
   </owl:Class>

   <!-- ========================================= -->
   <!-- GIPP XML Header                           -->
   <!-- ========================================= -->

   <!-- Example
   S2A_OPER_GIP_ATMIMA_MPC__20150605T094744_V20150622T000000_21000101T000000_B00.HDR
   -->
   <owl:Class rdf:about="&s2;gippTarXmlHeader">
      <rdfs:label xml:lang="en">Sentinel-2 Auxiliary GIPP Tar: XML Header</rdfs:label>
      <rdfs:comment xml:lang="en">
      </rdfs:comment>
      <rdfs:subClassOf rdf:resource="&s2;item"/>
      <rdfs:subClassOf rdf:resource="&drb;xml-content"/>
      <drb:signature rdf:parseType="Resource">
         <drb:nameMatch>(?i)S2[AB]_...._GIP_......_...._[0-9]{8}T[0-9]{6}_V[0-9]{8}T[0-9]{6}_[0-9]{8}T[0-9]{6}_...\.HDR</drb:nameMatch>
      </drb:signature>
   </owl:Class>

   <!-- ========================================= -->
   <!-- GIPP Data Block File                      -->
   <!-- ========================================= -->

   <!-- Example
   S2A_OPER_GIP_ATMIMA_MPC__20150605T094744_V20150622T000000_21000101T000000_B00.DBL
   -->
   <owl:Class rdf:about="&s2;gippTarDataBlockFile">
      <rdfs:label xml:lang="en">Sentinel-2 Auxiliary GIPP Tar: Data Block File</rdfs:label>
      <rdfs:comment xml:lang="en">
      </rdfs:comment>
      <rdfs:subClassOf rdf:resource="&s2;item"/>
      <drb:signature rdf:parseType="Resource">
         <drb:nameMatch>(?i)S2[AB]_...._GIP_......_...._[0-9]{8}T[0-9]{6}_V[0-9]{8}T[0-9]{6}_[0-9]{8}T[0-9]{6}_...\.DBL</drb:nameMatch>
      </drb:signature>
      <!--
      <drb:implementationIdentifier>sdf</drb:implementationIdentifier>
      <drb:schemaLocation>
      </drb:schemaLocation>
      -->
   </owl:Class>

</rdf:RDF>
